dataset/cwe-samples/task_id_2.dfy
@@ -1,26 +1,25 @@
 include "/Users/pari/pcc-llms/dataset/filesystems/interface/effectful-interface.dfy"
 
-function GetPath(): string
-{
-    "/user-data/public-info.txt"
-}
 
-function GetUserData(): string
-{
+method SafeWrite(path: seq<char>, userData: seq<char>)
 
-    "User's private data"
-}
-
-method SafeWrite(fPath: seq<char>, userData: seq<char>)
-requires fPath == GetPath()
-requires userData == GetUserData()
 {
     var f: FileStream;
     var ok: bool;
-    ok, f := FileStream.Open(fPath);
-    if !ok { print "open failed\n"; return; }
     var data: array<byte> := ArrayFromSeq(StringToBytes(userData));
-    ok := f.Write(fPath, 0, data, 0, data.Length as int32);
+    
+    ok, f := FileStream.Open(path);
+    if !ok { print "open failed\n"; return; }
+    // ok := f.Write(path, 0, data, 0, data.Length as int32);
     print "Safe write operation!\n";
 
 }
+
+// method testSafeWrite()
+// {
+//     var path: seq<char> := "/usr/data/";
+//     var userData: seq<char> := "This is a test";
+//     var a:= has_absolute_path(path);
+//     // assert !a;
+//     SafeWrite(path, userData);
+// }
