dataset/cwe-samples/task_id_3.dfy
@@ -1,7 +1,7 @@
 include "/Users/pari/pcc-llms/dataset/filesystems/interface/effectful-interface.dfy"
 function GetFilePath(): string
 {
-    "/user-data/public-key.txt"
+    "../../../user-data/public-key.txt"
 }
 
 method ReadFile(fPath: seq<char>)
@@ -12,6 +12,8 @@ requires fPath == GetFilePath()
     ok, f := FileStream.Open(fPath);
     if !ok { print "open failed\n"; return; }
     var data: array<byte> := new byte[100];
+    var pathTraversal := f.NoPathTraversal(fPath);
+    var isAbsolutePath := f.IsAbsolutePath(fPath);
     ok := f.Read(fPath, 0, data, 0, data.Length as int32);
     print "Safe Read operation!\n";
 }
